backend/Cminor_coop.v
@@ -349,4 +349,18 @@ apply Build_DecayCoreSem with (decaysem := cmin_coop_sem).
   apply CMin_decay. 
 Defined.
 
+Program Definition cmin_memsem : @MemSem genv CMin_core.
+Proof.
+eapply Build_MemSem with (csem := CMin_core_sem).
+  intros.
+  destruct CS; try apply mem_step_refl.
+  + eapply mem_step_free; eassumption.
+  + destruct vaddr; inv H1. eapply mem_step_store; eassumption.
+  + eapply mem_step_free; eassumption.
+  + eapply extcall_mem_step; eassumption.
+  + eapply mem_step_free; eassumption.
+  + eapply mem_step_free; eassumption.
+  + eapply mem_step_alloc; eassumption.
+Defined.
+
 End CMINOR_COOP.
